src/cbor/pulse/raw/everparse/CBOR.Pulse.API.Nondet.Type.fst
@@ -9,3 +9,5 @@ let cbor_nondet_array_iterator_t = I.iterator Raw.cbor_raw
 let cbor_nondet_map_iterator_t = I.iterator (Raw.cbor_map_entry Raw.cbor_raw)
 
 let cbor_nondet_map_entry_t = Raw.cbor_map_entry Raw.cbor_raw
+
+let cbor_nondet_array_append_cell_t = I.mixed_list Raw.cbor_raw
