src/cbor/pulse/CBOR.Pulse.API.Det.Dummy.fsti
@@ -4,3 +4,6 @@ module T = CBOR.Pulse.API.Det.Type
 
 inline_for_extraction
 val dummy_cbor_det_t (_: unit) : T.cbor_det_t
+
+inline_for_extraction
+val dummy_cbor_det_array_append_cell (_: unit) : T.cbor_det_array_append_cell_t
