src/cbor/pulse/CBOR.Pulse.API.Det.Type.fsti
@@ -7,3 +7,10 @@ val cbor_det_map_entry_t: Type0
 val cbor_det_array_iterator_t: Type0
 
 val cbor_det_map_iterator_t: Type0
+
+(* Abstract type of the scratch cells the application must pre-allocate
+   (as references) to call cbor_det_array_append. A fixed number (two) of
+   such references is required per append. The type is kept abstract; use
+   CBOR.Pulse.API.Det.Dummy.dummy_cbor_det_array_append_cell to initialize
+   the references. *)
+val cbor_det_array_append_cell_t: Type0
