src/cbor/pulse/CBOR.Pulse.API.Nondet.Dummy.fsti
@@ -1,0 +1,9 @@
+module CBOR.Pulse.API.Nondet.Dummy
+
+module T = CBOR.Pulse.API.Nondet.Type
+
+inline_for_extraction
+val dummy_cbor_nondet_t (_: unit) : T.cbor_nondet_t
+
+inline_for_extraction
+val dummy_cbor_nondet_array_append_cell (_: unit) : T.cbor_nondet_array_append_cell_t
