src/cbor/pulse/CBOR.Pulse.API.Nondet.Type.fsti
@@ -7,3 +7,10 @@ val cbor_nondet_array_iterator_t: Type0
 val cbor_nondet_map_iterator_t: Type0
 
 val cbor_nondet_map_entry_t: Type0
+
+(* Abstract type of the scratch cells the application must pre-allocate
+   (as references) to call cbor_nondet_array_append. A fixed number (two) of
+   such references is required per append. The type is kept abstract; use
+   CBOR.Pulse.API.Nondet.Dummy.dummy_cbor_nondet_array_append_cell to
+   initialize the references. *)
+val cbor_nondet_array_append_cell_t: Type0
